Checkpoint proofs for indirect blocks
Everything is proven, but needs to be cleaned up.

src/BlockPtr.v
@@ -42,27 +42,42 @@ Module Type BlockPtrSig.
 
   Parameter IRLen    : irec -> addr.       (* get length *)
   Parameter IRIndPtr : irec -> addr.       (* get indirect block pointer *)
+  Parameter IRDindPtr: irec -> addr.       (* doubly-indirect block pointer *)
+  Parameter IRTindPtr: irec -> addr.       (* triply-indirect block pointer *)
   Parameter IRBlocks : irec -> list waddr. (* get direct block numbers *)
   Parameter IRAttrs  : irec -> iattr.      (* get untouched attributes *)
 
   (* setters *)
   Parameter upd_len  : irec -> addr -> irec.
-  Parameter upd_irec : forall (r : irec) (len : addr) (ibptr : addr) (dbns : list waddr), irec.
+  Parameter upd_irec : forall (r : irec) (len : addr) (ibptr : addr)
+                                                      (dibptr : addr)
+                                                      (tibptr : addr)
+                                                      (dbns : list waddr), irec.
+
+  (* setter equivalence *)
+  Parameter upd_irec_eq_upd_len : forall ir len, goodSize addrlen len ->
+    upd_len ir len = upd_irec ir len (IRIndPtr ir) (IRDindPtr ir) (IRTindPtr ir) (IRBlocks ir).
 
   (* getter/setter lemmas *)
   Parameter upd_len_get_len    : forall ir n, goodSize addrlen n -> IRLen (upd_len ir n) = n.
   Parameter upd_len_get_ind    : forall ir n, IRIndPtr (upd_len ir n) = IRIndPtr ir.
+  Parameter upd_len_get_dind   : forall ir n, IRDindPtr (upd_len ir n) = IRDindPtr ir.
+  Parameter upd_len_get_tind   : forall ir n, IRTindPtr (upd_len ir n) = IRTindPtr ir.
   Parameter upd_len_get_blk    : forall ir n, IRBlocks (upd_len ir n) = IRBlocks ir.
   Parameter upd_len_get_iattr  : forall ir n, IRAttrs (upd_len ir n) = IRAttrs ir.
 
-  Parameter upd_irec_get_len   : forall ir len ibptr dbns,
-     goodSize addrlen len -> IRLen (upd_irec ir len ibptr dbns) = len.
-  Parameter upd_irec_get_ind   : forall ir len ibptr dbns,
-     goodSize addrlen ibptr -> IRIndPtr (upd_irec ir len ibptr dbns) = ibptr.
-  Parameter upd_irec_get_blk   : forall ir len ibptr dbns,
-     IRBlocks (upd_irec ir len ibptr dbns) = dbns.
-  Parameter upd_irec_get_iattr : forall ir len ibptr dbns,
-      IRAttrs (upd_irec ir len ibptr dbns) = IRAttrs ir.
+  Parameter upd_irec_get_len   : forall ir len ibptr dibptr tibptr dbns,
+     goodSize addrlen len -> IRLen (upd_irec ir len ibptr dibptr tibptr dbns) = len.
+  Parameter upd_irec_get_ind   : forall ir len ibptr dibptr tibptr dbns,
+     goodSize addrlen ibptr -> IRIndPtr (upd_irec ir len ibptr dibptr tibptr dbns) = ibptr.
+  Parameter upd_irec_get_dind  : forall ir len ibptr dibptr tibptr dbns,
+     goodSize addrlen dibptr -> IRDindPtr (upd_irec ir len ibptr dibptr tibptr dbns) = dibptr.
+  Parameter upd_irec_get_tind  : forall ir len ibptr dibptr tibptr dbns,
+     goodSize addrlen tibptr -> IRTindPtr (upd_irec ir len ibptr dibptr tibptr dbns) = tibptr.
+  Parameter upd_irec_get_blk   : forall ir len ibptr dibptr tibptr dbns,
+     IRBlocks (upd_irec ir len ibptr dibptr tibptr dbns) = dbns.
+  Parameter upd_irec_get_iattr : forall ir len ibptr dibptr tibptr dbns,
+      IRAttrs (upd_irec ir len ibptr dibptr tibptr dbns) = IRAttrs ir.
 
 End BlockPtrSig.
 
@@ -99,7 +114,7 @@ Module BlockPtr (BPtr : BlockPtrSig).
   Hint Extern 0 (okToUnify (IndRec.rep _ _) (IndRec.rep _ _)) => constructor : okToUnify.
 
   Notation "'NIndirect'" := IndSig.items_per_val.
-  Notation "'NBlocks'"   := (NDirect + NIndirect)%nat.
+  Notation "'NBlocks'"   := (NDirect + NIndirect + NIndirect ^ 2 + NIndirect ^ 3)%nat.
 
   (* Various bounds *)
   Lemma NIndirect_is : NIndirect = 512.
@@ -110,15 +125,18 @@ Module BlockPtr (BPtr : BlockPtrSig).
 
   Lemma NBlocks_roundtrip : # (natToWord addrlen NBlocks) = NBlocks.
   Proof.
-    unfold IndSig.items_per_val.
-    erewrite wordToNat_natToWord_bound with (bound:=$ valulen).
-    reflexivity.
-    eapply le_trans.
-    eapply plus_le_compat_r.
+    rewrite wordToNat_natToWord_idempotent. auto.
+    repeat rewrite Nat2N.inj_add.
+    simpl. repeat rewrite Nat2N.inj_mul. simpl.
+    rewrite NIndirect_is.
+    eapply N.le_lt_trans.
+    repeat rewrite <- N.add_assoc.
+    apply N.add_le_mono_r.
+    unfold N.le.
+    rewrite <- Nat2N.inj_compare.
+    apply nat_compare_le.
     apply NDirect_bound.
-    apply Nat.sub_0_le.
-    rewrite valulen_is.
-    compute; reflexivity.
+    compute. reflexivity.
   Qed.
 
   Lemma NDirect_roundtrip : # (natToWord addrlen NDirect) = NDirect.
@@ -158,7 +176,7 @@ Module BlockPtr (BPtr : BlockPtrSig).
 
   Local Hint Resolve le_ndirect_goodSize le_nindirect_goodSize le_nblocks_goodSize.
 
-  (************** rep invariant *)
+  (************** indirect blocks *)
 
    Definition indrep_n_helper bxp ibn iblocks :=
     (if (addr_eq_dec ibn 0)
@@ -179,68 +197,11 @@ Module BlockPtr (BPtr : BlockPtrSig).
     end)%pred.
 
   Hint Extern 0 (okToUnify (listmatch _ _ _) (listmatch _ _ _)) => constructor : okToUnify.
-  Hint Extern 0 (okToUnify (indrep_n_tree _ _ _ _ _) (indrep_n_tree _ _ _ _ _)) => constructor : okToUnify.
-
-  Definition indrep bxp ir (indlist : list waddr) nblocks :=
-    ( [[ nblocks = 0 ]] \/ (
-      [[ nblocks > 0 ]] * indrep_n_tree 0 bxp (IRIndPtr ir) indlist))%pred.
-
-  Definition rep bxp (ir : irec) (l : list waddr) :=
-    ( [[ length l = (IRLen ir) /\ length l <= NBlocks ]] *
-      [[ length (IRBlocks ir) = NDirect ]] *
-      exists indlist, indrep bxp ir indlist (length l - NDirect) *
-      [[ l = firstn (length l) ((IRBlocks ir) ++ indlist) ]] )%pred.
-
-  Definition rep_direct (ir : irec) (l : list waddr) : @pred _ addr_eq_dec valuset :=
-    ( [[ length l = (IRLen ir) /\ length l <= NBlocks /\ length l <= NDirect ]] *
-      [[ length (IRBlocks ir) = NDirect ]] *
-      [[ l = firstn (length l) (IRBlocks ir) ]] )%pred.
-
-  Definition rep_indirect bxp (ir : irec) (l : list waddr) :=
-    ( [[ length l = (IRLen ir) /\ length l <= NBlocks /\ length l > NDirect ]] *
-      [[ length (IRBlocks ir) = NDirect ]] *
-      exists indlist, indrep_n_tree 0 bxp (IRIndPtr ir) indlist *
-      [[ l = (IRBlocks ir) ++ firstn (length l - NDirect) indlist ]] )%pred.
+  Hint Extern 0 (okToUnify (indrep_n_tree _ _ _ _) (indrep_n_tree _ _ _ _ )) => constructor : okToUnify.
 
   (* Necessary to make subst work when there's a recursive term like:
      l = firstn (length l) ... *)
   Set Regular Subst Tactic.
-
-  Lemma rep_piff_direct : forall bxp ir l,
-    length l <= NDirect ->
-    rep bxp ir l <=p=> rep_direct ir l.
-  Proof.
-    unfold rep, indrep, rep_direct; intros; split; cancel; try omega.
-    rewrite firstn_app_l in H5 by omega; auto.
-    substl l at 1; rewrite firstn_app_l by omega; auto.
-    Unshelve.
-    eauto.
-  Qed.
-
-  Lemma rep_piff_indirect : forall bxp ir l,
-    length l > NDirect ->
-    rep bxp ir l <=p=> rep_indirect bxp ir l.
-  Proof.
-    unfold rep, indrep, rep_indirect; intros; split; cancel; try omega.
-    rewrite <- firstn_app_r; setoid_rewrite H3.
-    replace (NDirect + (length l - NDirect)) with (length l) by omega; auto.
-    substl l at 1; rewrite <- firstn_app_r. setoid_rewrite H3.
-    replace (NDirect + (length l - NDirect)) with (length l) by omega; auto.
-    Unshelve. exact nil.
-  Qed.
-
-  Lemma rep_selN_direct_ok : forall F bxp ir l m off,
-    (F * rep bxp ir l)%pred m ->
-    off < NDirect ->
-    off < length l ->
-    selN (IRBlocks ir) off $0 = selN l off $0.
-  Proof.
-    unfold rep, indrep; intros; destruct_lift H.
-    substl.
-    rewrite selN_firstn by auto.
-    rewrite selN_app1 by omega; auto.
-  Qed.
-
   Local Hint Resolve IndRec.Defs.items_per_val_not_0.
   Local Hint Resolve IndRec.Defs.items_per_val_gt_0'.
 
@@ -1058,6 +1019,8 @@ Module BlockPtr (BPtr : BlockPtrSig).
       exact $0.
   Qed.
 
+  Local Hint Extern 1 ({{_}} Bind (indget _ _ _ _ _ ) _) => apply indget_ok : prog.
+
   Fixpoint indread (indlvl : nat) lxp (ir : addr) ms :=
     If (addr_eq_dec ir 0) {
       Ret ^(ms, repeat $0 (NIndirect ^ S indlvl))
@@ -1125,6 +1088,9 @@ Module BlockPtr (BPtr : BlockPtrSig).
       - apply LOG.rep_hashmap_subset; eauto.
     Grab Existential Variables. all : eauto; split; solve [eauto | exact ($0)].
   Qed.
+
+  (* TODO put this after indread *)
+  Local Hint Extern 1 ({{_}} Bind (indread _ _ _ _ ) _) => apply indread_ok : prog.
 
   Fixpoint indclear_all indlvl lxp bxp root ms : prog (LOG.mstate * Cache.cachestate) :=
     If (addr_eq_dec root 0) {
@@ -1989,6 +1955,24 @@ Hint Rewrite le_plus_minus_r using auto.
       }
     }.
 
+  (* TODO move this *)
+  Lemma indrep_n_roundup_helper_1 : forall a b n, n <> 0 ->
+    n - a mod n < b -> roundup a n - a <= b.
+  Proof.
+    intros.
+    destruct (addr_eq_dec (a mod n) 0).
+    unfold roundup. rewrite divup_eq_div by auto. rewrite mul_div by mult_nonzero. omega.
+    rewrite roundup_eq by mult_nonzero. rewrite minus_plus. omega.
+  Qed.
+  Local Hint Resolve indrep_n_roundup_helper_1.
+
+  (* TODO move this *)
+  Theorem roundup_round : forall a n, roundup a n / n * n = roundup a n.
+  Proof.
+    intros.
+    destruct (Nat.eq_dec n 0). subst. unfold roundup. auto.
+    unfold roundup. rewrite Nat.div_mul by auto. auto.
+  Qed.
   Theorem indclear_ok : forall indlvl lxp bxp ir start len ms,
     {< F Fm m0 m l freelist,
     PRE:hm
@@ -2099,16 +2083,6 @@ Hint Rewrite le_plus_minus_r using auto.
         rewrite upd_range_length in *.
         repeat erewrite concat_hom_length in * by eauto.
         rewrite Nat.mul_cancel_r in * by mult_nonzero.
-        (* TODO move this *)
-        Lemma indrep_n_roundup_helper_1 : forall a b n, n <> 0 ->
-          n - a mod n < b -> roundup a n - a <= b.
-        Proof.
-          intros.
-          destruct (addr_eq_dec (a mod n) 0).
-          unfold roundup. rewrite divup_eq_div by auto. rewrite mul_div by mult_nonzero. omega.
-          rewrite roundup_eq by mult_nonzero. rewrite minus_plus. omega.
-        Qed.
-        Local Hint Resolve indrep_n_roundup_helper_1.
         destruct (addr_eq_dec (start mod N) 0).
         unfold roundup. rewrite divup_eq_div by auto. rewrite mul_div by mult_nonzero.
         autorewrite with core. eapply le_trans. apply div_add_distr_le. apply Nat.div_le_upper_bound; mult_nonzero.
@@ -2161,12 +2135,6 @@ Hint Rewrite le_plus_minus_r using auto.
         rewrite concat_hom_upd_range in * by eauto.
         replace I with (S indlvl) in * by omega.
         simpl in *. rewrite <- HeqN in *.
-        Theorem roundup_round : forall a n, roundup a n / n * n = roundup a n.
-        Proof.
-          intros.
-          destruct (Nat.eq_dec n 0). subst. unfold roundup. auto.
-          unfold roundup. rewrite Nat.div_mul by auto. auto.
-        Qed.
         rewrite roundup_round in * by mult_nonzero.
         rewrite upd_range_upd_range in *.
         rewrite listmatch_length_pimpl in *.
@@ -2292,33 +2260,6 @@ Hint Rewrite le_plus_minus_r using auto.
 
   Local Hint Extern 0 ({{_}} Bind (indput_get_blocks _ _ _ _) _) => apply indput_get_blocks_ok : prog.
 
-  (* This is an alternate spec for IndRec.write that does not require IndRec.rep
-    to hold beforehand. This allows blind writes to blocks that have not been
-    initialized beforehand with IndRec.init *)
-  Theorem IndRec_write_blind_ok : forall lxp xp items ms,
-    {< F Fm m0 m old,
-    PRE:hm
-          LOG.rep lxp F (LOG.ActiveTxn m0 m) ms hm *
-          [[ IndRec.items_valid xp items ]] * [[ xp <> 0 ]] *
-          [[[ m ::: Fm * arrayN (@ptsto _ addr_eq_dec _) xp [old] ]]]
-    POST:hm' RET:ms' exists m',
-          LOG.rep lxp F (LOG.ActiveTxn m0 m') ms' hm' *
-          [[[ m' ::: Fm * IndRec.rep xp items ]]]
-    CRASH:hm' LOG.intact lxp F m0 hm'
-    >} IndRec.write lxp xp items ms.
-  Proof.
-    unfold IndRec.write, IndRec.rep, IndRec.items_valid.
-    hoare.
-    unfold IndSig.RAStart. instantiate (1 := [_]). cancel.
-    rewrite IndRec.Defs.ipack_one. auto.
-    unfold IndRec.Defs.item in *. simpl in *. omega.
-    rewrite vsupsyn_range_synced_list; auto.
-    rewrite IndRec.Defs.ipack_one. auto.
-    unfold IndRec.Defs.item in *. simpl in *. omega.
-  Qed.
-
-  Local Hint Extern 0 ({{_}} Bind (IndRec.write _ _ _ _) _) => apply IndRec_write_blind_ok : prog.
-
   Fixpoint indput indlvl lxp bxp root off bn ms :=
     let N := NIndirect ^ indlvl in
     let is_alloc := (addr_eq_dec root 0) in
@@ -2359,130 +2300,227 @@ Hint Rewrite le_plus_minus_r using auto.
     f_equal. auto.
   Qed.
 
-  Theorem indput_ok : forall indlvl lxp bxp ir off bn ms,
-    {< F Fm m0 m l freelist,
-    PRE:hm
-           LOG.rep lxp F (LOG.ActiveTxn m0 m) ms hm *
-           [[[ m ::: (Fm * indrep_n_tree indlvl bxp ir l * BALLOC.rep bxp freelist) ]]] *
-           [[ off < length l ]]
-    POST:hm' RET:^(ms, ir')
-           exists m', LOG.rep lxp F (LOG.ActiveTxn m0 m') ms hm' *
-           ([[ ir' = 0 ]] \/
-           exists freelist' l',
-           [[ ir = 0 \/ ir = ir' ]] *
-           [[[ m' ::: (Fm * indrep_n_tree indlvl bxp ir' l' * BALLOC.rep bxp freelist') ]]] *
-           [[ incl freelist' freelist ]] * [[ l' = updN l off bn ]])
-    CRASH:hm'  LOG.intact lxp F m0 hm'
-    >} indput indlvl lxp bxp ir off bn ms.
+  (* putting this in a section prevents leaking the hint below to the global scope *)
+  Section indput_wrap.
+
+    (* This is an alternate spec for IndRec.write that does not require IndRec.rep
+      to hold beforehand. This allows blind writes to blocks that have not been
+      initialized beforehand with IndRec.init *)
+    Theorem IndRec_write_blind_ok : forall lxp xp items ms,
+      {< F Fm m0 m old,
+      PRE:hm
+            LOG.rep lxp F (LOG.ActiveTxn m0 m) ms hm *
+            [[ IndRec.items_valid xp items ]] * [[ xp <> 0 ]] *
+            [[[ m ::: Fm * arrayN (@ptsto _ addr_eq_dec _) xp [old] ]]]
+      POST:hm' RET:ms' exists m',
+            LOG.rep lxp F (LOG.ActiveTxn m0 m') ms' hm' *
+            [[[ m' ::: Fm * IndRec.rep xp items ]]]
+      CRASH:hm' LOG.intact lxp F m0 hm'
+      >} IndRec.write lxp xp items ms.  
     Proof.
-      induction indlvl; intros; simpl.
-      + step.
-        - hoare.
-          --  unfold IndRec.items_valid, IndSig.RAStart, IndSig.RALen, IndSig.xparams_ok.
-              rewrite mult_1_l. unfold Rec.well_formed. simpl. unfold BALLOC.bn_valid in *.
-              rewrite length_updN, repeat_length. intuition.
-          --  unfold BALLOC.bn_valid in *. intuition.
-          --  or_r. cancel. unfold BALLOC.bn_valid in *; intuition.
-              rewrite indrep_n_helper_0. rewrite indrep_n_helper_valid by omega.
-              unfold BALLOC.bn_valid. cancel.
-        - hoare.
-        --  rewrite indrep_n_helper_valid by omega. cancel.
-        --  or_r. cancel.
-            rewrite indrep_n_helper_valid in * by omega. cancel.
-            match goal with [H : context [?P] |- ?P] => destruct_lift H end. auto.
-      + step.
-        - step. safestep.
-          rewrite repeat_selN, roundTrip_0. rewrite indrep_n_helper_0, indrep_n_tree_0. cancel.
-          indrep_n_tree_bound.
-          rewrite repeat_length. apply Nat.mod_bound_pos; mult_nonzero; omega.
-          unfold indput_upd_if_necessary.
-          rewrite repeat_selN. rewrite roundTrip_0.
-          hoare.
-          unfold BALLOC.bn_valid in *.
-          unfold IndRec.items_valid, IndSig.xparams_ok, IndSig.RAStart, IndSig.RALen, Rec.well_formed.
-          simpl. rewrite length_updN, repeat_length. intuition.
-          unfold BALLOC.bn_valid in *. intuition.
-          or_r.
-          (* safecancel isn't safe enough, so do it manually - the long and short of it is that the
-             listmatches get canceled before the indrep_n_helper, causing incorrect instantiation *)
-          norm. cancel. repeat split; auto.
-          pred_apply. norm; intuition. instantiate (iblocks := updN _ _ _). cancel.
-          unfold BALLOC.bn_valid in *; intuition.
-          rewrite indrep_n_helper_valid by omega. cancel.
-          rewrite listmatch_updN_removeN.
-          indrep_n_extract. cancel.
-          rewrite repeat_selN, roundTrip_0. rewrite indrep_n_tree_0.
-          rewrite wordToNat_natToWord_idempotent'. cancel.
-          eapply BALLOC.bn_valid_goodSize; eauto.
-          rewrite indrep_n_tree_valid in * by auto. destruct_lifts. auto.
-          all : try rewrite repeat_length.
-          all : try solve [indrep_n_tree_bound].
-          unfold BALLOC.bn_valid. auto.
-          erewrite Nat.div_mod with (x := off) at 1.
-          rewrite plus_comm, mult_comm. rewrite updN_concat. f_equal.
-          match goal with [H : context [?l] |- context [selN ?l] ] =>
-            rewrite listmatch_extract with (b := l) in H
-          end. rewrite repeat_selN in *. rewrite roundTrip_0, indrep_n_tree_0 in *.
-          destruct_lifts.
-          match goal with [H : selN _ _ _ = _ |- _] => rewrite H end. reflexivity.
-          all : try rewrite repeat_length.
-          all : try solve [indrep_n_tree_bound].
-          apply Nat.mod_bound_pos; mult_nonzero; omega.
-          eapply indrep_n_indlist_forall_length.
-          match goal with [H : context [listmatch _ _ ?l] |- context [listmatch _ _ ?l] ] =>
-            eapply pimpl_apply; [> |exact H]; cancel end. rewrite indrep_n_helper_0. cancel.
-          mult_nonzero.
-          auto.
-          cancel.
-          or_l. cancel.
-        - step.
-          rewrite indrep_n_helper_valid in * by auto. destruct_lifts. eauto.
-          cancel. cancel_last.
-          safestep.
-          indrep_n_extract; solve [cancel_last | indrep_n_tree_bound].
-          eapply lt_le_trans.
-          apply Nat.mod_bound_pos; mult_nonzero; omega.
-          apply Nat.eq_le_incl. symmetry. apply Forall_selN.
-          eapply indrep_n_indlist_forall_length.
-          match goal with [H : context [listmatch _ _ ?l] |- context [listmatch _ _ ?l] ] =>
-            eapply pimpl_apply; [> |exact H]; cancel end. cancel_last.
-          indrep_n_tree_bound.
-          hoare.
-        --  rewrite indrep_n_helper_valid in * by omega. destruct_lifts. auto.
-        --  or_r.
-            norm. cancel. repeat (split; try reflexivity). auto.
-            pred_apply. norm; intuition.
-            instantiate (iblocks := updN _ _ _). cancel.
-            rewrite listmatch_updN_removeN by indrep_n_tree_bound. cancel.
-            rewrite wordToNat_natToWord_idempotent'. cancel. apply pimpl_refl.
+      unfold IndRec.write, IndRec.rep, IndRec.items_valid.
+      hoare.
+      unfold IndSig.RAStart. instantiate (1 := [_]). cancel.
+      rewrite IndRec.Defs.ipack_one. auto.
+      unfold IndRec.Defs.item in *. simpl in *. omega.
+      rewrite vsupsyn_range_synced_list; auto.
+      rewrite IndRec.Defs.ipack_one. auto.
+      unfold IndRec.Defs.item in *. simpl in *. omega.
+    Qed.
+
+    Local Hint Extern 0 ({{_}} Bind (IndRec.write _ _ _ _) _) => apply IndRec_write_blind_ok : prog.
+
+    Theorem indput_ok : forall indlvl lxp bxp ir off bn ms,
+      {< F Fm m0 m l freelist,
+      PRE:hm
+             LOG.rep lxp F (LOG.ActiveTxn m0 m) ms hm *
+             [[[ m ::: (Fm * indrep_n_tree indlvl bxp ir l * BALLOC.rep bxp freelist) ]]] *
+             [[ off < length l ]]
+      POST:hm' RET:^(ms, ir')
+             exists m', LOG.rep lxp F (LOG.ActiveTxn m0 m') ms hm' *
+             ([[ ir' = 0 ]] \/
+             exists freelist' l',
+             [[ ir = 0 \/ ir = ir' ]] *
+             [[[ m' ::: (Fm * indrep_n_tree indlvl bxp ir' l' * BALLOC.rep bxp freelist') ]]] *
+             [[ incl freelist' freelist ]] * [[ l' = updN l off bn ]])
+      CRASH:hm'  LOG.intact lxp F m0 hm'
+      >} indput indlvl lxp bxp ir off bn ms.
+      Proof.
+        induction indlvl; intros; simpl.
+        + step.
+          - hoare.
+            --  unfold IndRec.items_valid, IndSig.RAStart, IndSig.RALen, IndSig.xparams_ok.
+                rewrite mult_1_l. unfold Rec.well_formed. simpl. unfold BALLOC.bn_valid in *.
+                rewrite length_updN, repeat_length. intuition.
+            --  unfold BALLOC.bn_valid in *. intuition.
+            --  or_r. cancel. unfold BALLOC.bn_valid in *; intuition.
+                rewrite indrep_n_helper_0. rewrite indrep_n_helper_valid by omega.
+                unfold BALLOC.bn_valid. cancel.
+          - hoare.
+          --  rewrite indrep_n_helper_valid by omega. cancel.
+          --  or_r. cancel.
+              rewrite indrep_n_helper_valid in * by omega. cancel.
+              match goal with [H : context [?P] |- ?P] => destruct_lift H end. auto.
+        + step.
+          - step. safestep.
+            rewrite repeat_selN, roundTrip_0. rewrite indrep_n_helper_0, indrep_n_tree_0. cancel.
+            indrep_n_tree_bound.
+            rewrite repeat_length. apply Nat.mod_bound_pos; mult_nonzero; omega.
+            unfold indput_upd_if_necessary.
+            rewrite repeat_selN. rewrite roundTrip_0.
+            hoare.
+            unfold BALLOC.bn_valid in *.
+            unfold IndRec.items_valid, IndSig.xparams_ok, IndSig.RAStart, IndSig.RALen, Rec.well_formed.
+            simpl. rewrite length_updN, repeat_length. intuition.
+            unfold BALLOC.bn_valid in *. intuition.
+            or_r.
+            (* safecancel isn't safe enough, so do it manually - the long and short of it is that the
+               listmatches get canceled before the indrep_n_helper, causing incorrect instantiation *)
+            norm. cancel. repeat split; auto.
+            pred_apply. norm; intuition. instantiate (iblocks := updN _ _ _). cancel.
+            unfold BALLOC.bn_valid in *; intuition.
+            rewrite indrep_n_helper_valid by omega. cancel.
+            rewrite listmatch_updN_removeN.
+            indrep_n_extract. cancel.
+            rewrite repeat_selN, roundTrip_0. rewrite indrep_n_tree_0.
+            rewrite wordToNat_natToWord_idempotent'. cancel.
             eapply BALLOC.bn_valid_goodSize; eauto.
             rewrite indrep_n_tree_valid in * by auto. destruct_lifts. auto.
+            all : try rewrite repeat_length.
+            all : try solve [indrep_n_tree_bound].
+            unfold BALLOC.bn_valid. auto.
             erewrite Nat.div_mod with (x := off) at 1.
-            rewrite plus_comm, mult_comm. rewrite updN_concat. reflexivity.
+            rewrite plus_comm, mult_comm. rewrite updN_concat. f_equal.
+            match goal with [H : context [?l] |- context [selN ?l] ] =>
+              rewrite listmatch_extract with (b := l) in H
+            end. rewrite repeat_selN in *. rewrite roundTrip_0, indrep_n_tree_0 in *.
+            destruct_lifts.
+            match goal with [H : selN _ _ _ = _ |- _] => rewrite H end. reflexivity.
+            all : try rewrite repeat_length.
+            all : try solve [indrep_n_tree_bound].
             apply Nat.mod_bound_pos; mult_nonzero; omega.
             eapply indrep_n_indlist_forall_length.
             match goal with [H : context [listmatch _ _ ?l] |- context [listmatch _ _ ?l] ] =>
-              eapply pimpl_apply; [> |exact H]; cancel end. cancel_last.
+              eapply pimpl_apply; [> |exact H]; cancel end. rewrite indrep_n_helper_0. cancel.
             mult_nonzero.
             auto.
-        --  rewrite indrep_n_helper_valid in * by omega. destruct_lifts. auto.
-        --  or_r.
-            norm. cancel. repeat split. auto.
-            pred_apply. norm; intuition.
-            instantiate (iblocks := updN _ _ _). cancel.
-            rewrite listmatch_updN_removeN by indrep_n_tree_bound. cancel.
-            rewrite natToWord_wordToNat. cancel. apply pimpl_refl.
-            erewrite Nat.div_mod with (x := off) at 1.
-            rewrite plus_comm, mult_comm. rewrite updN_concat. reflexivity.
+            cancel.
+            or_l. cancel.
+          - step.
+            rewrite indrep_n_helper_valid in * by auto. destruct_lifts. eauto.
+            cancel. cancel_last.
+            safestep.
+            indrep_n_extract; solve [cancel_last | indrep_n_tree_bound].
+            eapply lt_le_trans.
             apply Nat.mod_bound_pos; mult_nonzero; omega.
+            apply Nat.eq_le_incl. symmetry. apply Forall_selN.
             eapply indrep_n_indlist_forall_length.
             match goal with [H : context [listmatch _ _ ?l] |- context [listmatch _ _ ?l] ] =>
               eapply pimpl_apply; [> |exact H]; cancel end. cancel_last.
-            mult_nonzero.
-            auto.
-        --  cancel.
-    Grab Existential Variables. all : auto; solve [exact nil | exact $0].
+            indrep_n_tree_bound.
+            hoare.
+          --  rewrite indrep_n_helper_valid in * by omega. destruct_lifts. auto.
+          --  or_r.
+              norm. cancel. repeat (split; try reflexivity). auto.
+              pred_apply. norm; intuition.
+              instantiate (iblocks := updN _ _ _). cancel.
+              rewrite listmatch_updN_removeN by indrep_n_tree_bound. cancel.
+              rewrite wordToNat_natToWord_idempotent'. cancel. apply pimpl_refl.
+              eapply BALLOC.bn_valid_goodSize; eauto.
+              rewrite indrep_n_tree_valid in * by auto. destruct_lifts. auto.
+              erewrite Nat.div_mod with (x := off) at 1.
+              rewrite plus_comm, mult_comm. rewrite updN_concat. reflexivity.
+              apply Nat.mod_bound_pos; mult_nonzero; omega.
+              eapply indrep_n_indlist_forall_length.
+              match goal with [H : context [listmatch _ _ ?l] |- context [listmatch _ _ ?l] ] =>
+                eapply pimpl_apply; [> |exact H]; cancel end. cancel_last.
+              mult_nonzero.
+              auto.
+          --  rewrite indrep_n_helper_valid in * by omega. destruct_lifts. auto.
+          --  or_r.
+              norm. cancel. repeat split. auto.
+              pred_apply. norm; intuition.
+              instantiate (iblocks := updN _ _ _). cancel.
+              rewrite listmatch_updN_removeN by indrep_n_tree_bound. cancel.
+              rewrite natToWord_wordToNat. cancel. apply pimpl_refl.
+              erewrite Nat.div_mod with (x := off) at 1.
+              rewrite plus_comm, mult_comm. rewrite updN_concat. reflexivity.
+              apply Nat.mod_bound_pos; mult_nonzero; omega.
+              eapply indrep_n_indlist_forall_length.
+              match goal with [H : context [listmatch _ _ ?l] |- context [listmatch _ _ ?l] ] =>
+                eapply pimpl_apply; [> |exact H]; cancel end. cancel_last.
+              mult_nonzero.
+              auto.
+          --  cancel.
+      Grab Existential Variables. all : auto; solve [exact nil | exact $0].
+    Qed.
+
+  End indput_wrap.
+
+  Local Hint Extern 0 ({{_}} Bind (indput _ _ _ _ _ _ _) _) => apply indput_ok : prog.
+
+  (************** rep invariant *)
+
+  Definition indrep bxp ir (indlist : list waddr) :=
+    ( indrep_n_tree 0 bxp (IRIndPtr ir) (firstn NIndirect indlist) *
+      indrep_n_tree 1 bxp (IRDindPtr ir) (firstn (NIndirect ^ 2) (skipn NIndirect indlist)) *
+      indrep_n_tree 2 bxp (IRTindPtr ir) (skipn (NIndirect + NIndirect ^ 2) indlist)
+    )%pred.
+
+  Opaque indrep_n_tree.
+
+  Definition rep bxp (ir : irec) (l : list waddr) :=
+    ( [[ length l = (IRLen ir) /\ length l <= NBlocks ]] *
+      [[ length (IRBlocks ir) = NDirect ]] *
+      exists indlist, indrep bxp ir indlist *
+      [[ l = firstn (length l) ((IRBlocks ir) ++ indlist) ]] )%pred.
+
+  Definition rep_direct bxp (ir : irec) (l : list waddr) : @pred _ addr_eq_dec valuset :=
+    ( [[ length l = (IRLen ir) /\ length l <= NBlocks /\ length l <= NDirect ]] *
+      [[ length (IRBlocks ir) = NDirect ]] *
+      exists indlist, indrep bxp ir indlist *
+      [[ l = firstn (length l) (IRBlocks ir) ]] )%pred.
+
+  Definition rep_indirect bxp (ir : irec) (l : list waddr) :=
+    ( [[ length l = (IRLen ir) /\ length l <= NBlocks /\ length l > NDirect ]] *
+      [[ length (IRBlocks ir) = NDirect ]] *
+      exists indlist, indrep bxp ir indlist *
+      [[ l = (IRBlocks ir) ++ firstn (length l - NDirect) indlist ]] )%pred.
+
+  Lemma rep_piff_direct : forall bxp ir l,
+    length l <= NDirect ->
+    rep bxp ir l <=p=> rep_direct bxp ir l.
+  Proof.
+    intros. unfold rep, rep_direct. split; cancel.
+    replace (length l - NDirect) with 0 by omega. cancel.
+    rewrite firstn_app_l in * by omega; auto.
+    replace (length l - NDirect) with 0 by omega. cancel.
+    substl l at 1; rewrite firstn_app_l by omega; auto.
   Qed.
+
+  Lemma rep_piff_indirect : forall bxp ir l,
+    length l > NDirect ->
+    rep bxp ir l <=p=> rep_indirect bxp ir l.
+  Proof.
+    unfold rep, rep_indirect; intros; split; cancel; try omega.
+    rewrite <- firstn_app_r; setoid_rewrite H3.
+    replace (NDirect + (length l - NDirect)) with (length l) by omega; auto.
+    substl l at 1; rewrite <- firstn_app_r. setoid_rewrite H3.
+    replace (NDirect + (length l - NDirect)) with (length l) by omega; auto.
+  Qed.
+
+  Lemma rep_selN_direct_ok : forall F bxp ir l m off,
+    (F * rep bxp ir l)%pred m ->
+    off < NDirect ->
+    off < length l ->
+    selN (IRBlocks ir) off $0 = selN l off $0.
+  Proof.
+    unfold rep. intros; destruct_lift H.
+    substl.
+    rewrite selN_firstn by auto.
+    rewrite selN_app1 by omega; auto.
+  Qed.
+
 
   (************* program *)
 
@@ -2490,92 +2528,94 @@ Hint Rewrite le_plus_minus_r using auto.
     If (lt_dec off NDirect) {
       Ret ^(ms, selN (IRBlocks ir) off $0)
     } else {
-      let^ (ms, v) <- indget 0 lxp (IRIndPtr ir) (off - NDirect) ms;
-      Ret ^(ms, v)
+      let off := off - NDirect in
+      If (lt_dec off NIndirect) {
+        indget 0 lxp (IRIndPtr ir) off ms
+      } else {
+        let off := off - NIndirect in
+        If (lt_dec off (NIndirect ^ 2)) {
+          indget 1 lxp (IRDindPtr ir) off ms
+        } else {
+          let off := off - NIndirect ^ 2 in
+          indget 2 lxp (IRTindPtr ir) off ms
+        }
+      }
     }.
 
   Definition read lxp (ir : irec) ms :=
     If (le_dec (IRLen ir) NDirect) {
       Ret ^(ms, firstn (IRLen ir) (IRBlocks ir))
     } else {
-      let^ (ms, indbns) <- indread 0 lxp (IRIndPtr ir) (IRLen ir - NDirect) ms;
-      Ret ^(ms, (firstn (IRLen ir) ((IRBlocks ir) ++ indbns)))
+      let^ (ms, indbns) <- indread 0 lxp (IRIndPtr ir) ms;
+      let^ (ms, dindbns) <- indread 1 lxp (IRDindPtr ir) ms;
+      let^ (ms, tindbns) <- indread 2 lxp (IRTindPtr ir) ms;
+      Ret ^(ms, (firstn (IRLen ir) ((IRBlocks ir) ++ indbns ++ dindbns ++ tindbns)))
     }.
 
-  Definition free_ind_dec ol nl :
-    { ol > NDirect /\ nl <= NDirect } + { ol <= NDirect \/ nl > NDirect }.
-  Proof.
-    destruct (gt_dec ol NDirect).
-    destruct (le_dec nl NDirect).
-    left; split; assumption.
-    right; right; apply not_le; assumption.
-    right; left; apply not_gt; assumption.
-  Defined.
+  Definition indshrink_helper indlvl lxp bxp bn nl ms :=
+    let start := fold_left plus (map (fun i => NIndirect ^ S i) (seq 0 indlvl)) 0 in
+    let len := NIndirect ^ S indlvl in
+    If (lt_dec nl (start + len)) {
+      indclear indlvl lxp bxp bn (nl - start) (len - (nl - start)) ms
+    } else {
+      Ret ^(ms, bn)
+    }.
 
+  Definition indshrink lxp bxp ir nl ms :=
+    let^ (ms, indptr)  <- indshrink_helper 0 lxp bxp (IRIndPtr ir)  nl ms;
+    let^ (ms, dindptr) <- indshrink_helper 1 lxp bxp (IRDindPtr ir) nl ms;
+    let^ (ms, tindptr) <- indshrink_helper 2 lxp bxp (IRTindPtr ir) nl ms;
+    Ret ^(ms, indptr, dindptr, tindptr).
 
   Definition shrink lxp bxp (ir : irec) nr ms :=
-    let nl := ((IRLen ir) - nr) in
-    If (free_ind_dec (IRLen ir) nl) {
-      ms <- BALLOC.free lxp bxp (IRIndPtr ir) ms;
+    let ol := (IRLen ir) in
+    let nl := (ol - nr) in
+    If (le_dec ol NDirect) {
       Ret ^(ms, upd_len ir nl)
     } else {
-      Ret ^(ms, upd_len ir nl)
+      let ol' := ol - NDirect in
+      let nl' := nl - NDirect in
+      let^ (ms, indptr, dindptr, tindptr) <- indshrink lxp bxp ir nl' ms;
+      Ret ^(ms, upd_irec ir nl indptr dindptr tindptr (IRBlocks ir))
     }.
 
+  Definition indgrow lxp bxp ir off bn ms :=
+    If (lt_dec off NIndirect) {
+      let^ (ms, v) <- indput 0 lxp bxp (IRIndPtr ir) off bn ms;
+      Ret ^(ms, v, v, (IRDindPtr ir), (IRTindPtr ir))
+    } else {
+      let off := off - NIndirect in
+      If (lt_dec off (NIndirect ^ 2)) {
+        let^ (ms, v) <- indput 1 lxp bxp (IRDindPtr ir) off bn ms;
+        Ret ^(ms, v, (IRIndPtr ir), v, (IRTindPtr ir))
+      } else {
+        let off := off - NIndirect ^ 2 in
+        let^ (ms, v) <- indput 2 lxp bxp (IRTindPtr ir) off bn ms;
+        Ret ^(ms, v, (IRIndPtr ir), (IRDindPtr ir), v)
+      }
+    }.
 
   Definition grow lxp bxp (ir : irec) bn ms :=
     let len := (IRLen ir) in
     If (lt_dec len NDirect) {
       (* change direct block address *)
-      Ret ^(ms, Some (upd_irec ir (S len) (IRIndPtr ir) (updN (IRBlocks ir) len bn)))
+      Ret ^(ms, Some (upd_irec ir (S len) (IRIndPtr ir) (IRDindPtr ir) (IRTindPtr ir) (updN (IRBlocks ir) len bn)))
     } else {
-      (* allocate indirect block if necessary *)
-      let^ (ms, ibn) <- If (addr_eq_dec len NDirect) {
-        let^ (ms, r) <- BALLOC.alloc lxp bxp ms;
-        match r with
-        | None => Ret ^(ms, None)
-        | Some ibn =>
-            ms <- IndRec.init lxp ibn ms;
-            Ret ^(ms, Some ibn)
-        end
+      let off := (len - NDirect) in
+      If (waddr_eq_dec bn $0) {
+        let^ (ms, indptr, dindptr, tindptr) <- indshrink lxp bxp ir off ms;
+        Ret ^(ms, Some (upd_irec ir (S len) indptr dindptr tindptr (IRBlocks ir)))
       } else {
-        Ret ^(ms, Some (IRIndPtr ir))
-      };
-      match ibn with
-      | Some ibn =>
-        (* write indirect block *)
-        ms <- IndRec.put lxp ibn (len - NDirect) bn ms;
-        Ret ^(ms, Some (upd_irec ir (S len) ibn (IRBlocks ir)))
-      | None => Ret ^(ms, None)
-      end
+        let^ (ms, v, indptr, dindptr, tindptr) <- indgrow lxp bxp ir off bn ms;
+        If (addr_eq_dec v 0) {
+          Ret ^(ms, None)
+        } else {
+          Ret ^(ms, Some (upd_irec ir (S len) indptr dindptr tindptr (IRBlocks ir)))
+        }
+      }
     }.
 
-  Fact div_mod_le : forall a b, b <> 0 -> a mod b + a / b * b <= a.
-  Proof.
-    intros.
-    destruct (le_lt_dec (a mod b) 0).
-    rewrite mul_div; omega.
-    rewrite mult_comm, plus_comm.
-    rewrite <- Nat.div_mod; omega.
-  Qed.
-
-  Fact sub_mult_bound : forall n a b c, b >= c * n -> a < c -> b - a * n >= n.
-  Proof.
-    intros.
-    remember (c - a) as e. assert (c = a + e) by omega; subst c.
-    rewrite Nat.mul_add_distr_r in *.
-    assert (1 <= e) by omega.
-    assert (n <= e * n).
-    rewrite <- mult_1_l at 1.
-    apply mult_le_compat_r; auto.
-    lia.
-  Qed.
-
-  Hint Rewrite length_enumerate firstn_enumerate : list.
-
-  Opaque indget.
-  Hint Extern 1 ({{_}} Bind (indget _ _ _ _ _) _) => apply indget_ok : prog.
-  Hint Extern 1 ({{_}} Bind (indread _ _ _ _) _) => apply indread_ok : prog.
+  Opaque indget indread indput indclear.
 
   Theorem get_ok : forall lxp bxp ir off ms,
     {< F Fm m0 m l,
@@ -2594,17 +2634,22 @@ Hint Rewrite le_plus_minus_r using auto.
     step.
     step.
     eapply rep_selN_direct_ok; eauto.
-
     prestep; norml.
-    rewrite rep_piff_indirect in H0 by omega.
-    unfold rep_indirect in H0; destruct_lift H0; cancel; try omega.
-    eassumption.
-    step; substl.
-    substl NDirect; rewrite selN_app2.
-    rewrite selN_firstn by omega; auto.
-    omega.
+    rewrite rep_piff_indirect in * by omega.
+    unfold rep_indirect, indrep in *. destruct_lifts.
+    hoare; match goal with
+    | [H : context [indrep_n_tree _ _ _ ?L] |- _ < length ?L] =>
+      rewrite indrep_n_length_pimpl with (l := L) in H; destruct_lift H; omega
+    | [ |- pimpl _ _] => cancel; cancel_last
+    | [|- ?H] => idtac H
+    end.
+    - substl l. rewrite selN_app2. repeat rewrite selN_firstn.
+      f_equal. all: omega.
+    - substl l. rewrite selN_app2. repeat rewrite selN_firstn.
+      rewrite skipn_selN. f_equal. all : omega.
+    - substl l. rewrite selN_app2. repeat rewrite selN_firstn.
+      rewrite skipn_selN. f_equal. all : omega.
   Qed.
-
 
   Theorem read_ok : forall lxp bxp ir ms,
     {< F Fm m0 m l,
@@ -2625,17 +2670,17 @@ Hint Rewrite le_plus_minus_r using auto.
     substl; substl (length l); auto.
     unfold rep in H; destruct_lift H; omega.
 
-    prestep; norml.
-    rewrite rep_piff_indirect in Hx.
-    unfold rep_indirect in Hx; destruct_lift Hx; cancel.
-    step; substl.
-    rewrite Nat.add_0_r, firstn_app_le by omega.
-    setoid_rewrite firstn_oob at 2; try omega.
-    substl (length l); substl NDirect; auto.
-    unfold rep in Hx; destruct_lift Hx; omega.
+    unfold rep, indrep in Hx. destruct_lifts.
+    hoare; match goal with
+    | [H : context [indrep_n_tree _ _ _ ?L] |- _ < length ?L] =>
+      rewrite indrep_n_length_pimpl with (l := L) in H; destruct_lift H; omega
+    | [ |- pimpl _ _] => cancel; cancel_last
+    | [|- ?H] => idtac H
+    end.
+    rewrite app_assoc with (l := firstn _ _).
+    rewrite <- firstn_sum_split. rewrite firstn_skipn.
+    congruence.
   Qed.
-
-
 
   Lemma indrec_ptsto_pimpl : forall ibn indrec,
     IndRec.rep ibn indrec =p=> exists v, ibn |-> (v, nil).
@@ -2647,7 +2692,6 @@ Hint Rewrite le_plus_minus_r using auto.
     rewrite IndRec.Defs.ipack_length.
     setoid_rewrite H0.
     rewrite Rounding.divup_mul; auto.
-    apply IndRec.Defs.items_per_val_not_0.
 
     rewrite arrayN_isolate with (i := 0) by omega.
     unfold IndSig.RAStart; rewrite Nat.add_0_r.
@@ -2657,70 +2701,259 @@ Hint Rewrite le_plus_minus_r using auto.
   Qed.
 
   Hint Rewrite cuttail_length : core.
-  Hint Rewrite upd_len_get_len upd_len_get_ind upd_len_get_blk upd_len_get_iattr : core.
-  Hint Rewrite upd_irec_get_len upd_irec_get_ind upd_irec_get_blk upd_irec_get_iattr : core.
+  Hint Rewrite upd_len_get_len upd_len_get_ind upd_len_get_dind upd_len_get_tind upd_len_get_blk upd_len_get_iattr : core.
+  Hint Rewrite upd_irec_get_len upd_irec_get_ind upd_irec_get_dind upd_irec_get_tind upd_irec_get_blk upd_irec_get_iattr : core.
   Local Hint Resolve upd_len_get_iattr upd_irec_get_iattr.
+
+  Theorem upd_len_indrep : forall bxp ir l n,
+    indrep bxp ir l <=p=> indrep bxp (upd_len ir n) l.
+  Proof.
+    intros.
+    unfold indrep. autorewrite with core. auto.
+  Qed.
+
+  (* TODO move near indclear *)
+    Local Hint Extern 1 ({{_}} Bind (indclear _ _ _ _ _ _ _ ) _) => apply indclear_ok : prog.
+
+(* TODO move this *)
+  Ltac min_cases :=
+    let H := fresh in let H' := fresh in
+    edestruct Min.min_spec as [ [H H']|[H H'] ];
+    rewrite H' in *; clear H'.
+(* TODO move this *)
+  Lemma firstn_upd_range : forall T l n n' len (v : T),
+    n <= n' -> n <= length l -> firstn n (upd_range l n' len v) = firstn n l.
+  Proof.
+    intros. unfold upd_range. rewrite firstn_app_l.
+    rewrite firstn_firstn. rewrite Nat.min_comm.
+    min_cases; auto; omega.
+    rewrite firstn_length. min_cases; omega.
+  Qed.
+
+  Lemma firstn_eq_firstn_ge : forall T (l1 l2 : list T) n1 n2,
+    firstn n2 l1 = firstn n2 l2 -> n1 <= n2 -> firstn n1 l1 = firstn n1 l2.
+  Proof.
+    intros.
+    destruct (lt_dec (length l1) n2). rewrite firstn_oob in * by omega.
+    subst. rewrite firstn_firstn, min_l by omega. auto.
+    rewrite <- firstn_skipn with (n := n2) (l := l1).
+    rewrite <- firstn_skipn with (n := n2) (l := l2).
+    repeat rewrite firstn_app_l. congruence.
+    rewrite firstn_length. min_cases; try omega.
+    match goal with [H : firstn _ _ = firstn _ _|- _] =>
+      apply f_equal with (f := @length _) (x := firstn n2 l1) in H end.
+    repeat rewrite firstn_length in *. repeat min_cases; omega.
+    rewrite firstn_length. min_cases; omega.
+  Qed.
+
+  Theorem indshrink_helper_ok : forall lxp bxp bn nl indlvl ms,
+    let start := fold_left plus (map (fun i => NIndirect ^ S i) (seq 0 indlvl)) 0 in
+    {< F Fm m0 m l freelist,
+    PRE:hm
+           LOG.rep lxp F (LOG.ActiveTxn m0 m) ms hm *
+           [[[ m ::: (Fm * indrep_n_tree indlvl bxp bn l * BALLOC.rep bxp freelist) ]]]
+    POST:hm' RET:^(ms, r)  exists m' freelist' l',
+           LOG.rep lxp F (LOG.ActiveTxn m0 m') ms hm' *
+           [[[ m' ::: (Fm * indrep_n_tree indlvl bxp r l' * BALLOC.rep bxp freelist') ]]] *
+           [[ l' = upd_range l (nl - start) (length l - (nl - start)) $0 ]] * [[ incl freelist freelist' ]]
+    CRASH:hm'  LOG.intact lxp F m0 hm'
+    >} indshrink_helper indlvl lxp bxp bn nl ms.
+  Proof.
+    unfold indshrink_helper.
+    prestep. norml.
+    rewrite indrep_n_length_pimpl in *. destruct_lifts.
+    hoare.
+    replace (_ - (_ - _)) with 0 by omega. rewrite upd_range_0. auto.
+  Qed.
+
+  Local Hint Extern 1 ({{_}} Bind (indshrink_helper _ _ _ _ _ _ ) _) => apply indshrink_helper_ok : prog.
+
+  Ltac indrep_n_tree_extract_lengths :=
+    repeat match goal with [H : context [indrep_n_tree _ _ _ ?x] |- _] =>
+      match goal with
+      | [H' : length x = _ |- _] => fail 1
+      | [|- _] => rewrite indrep_n_length_pimpl with (l := x) in H; destruct_lift H
+      end
+    end; rewrite mult_1_r in *.
+
+(*TODO move this *)
+  Theorem indrep_length_pimpl : forall bxp ir l, indrep bxp ir l <=p=> indrep bxp ir l * [[ length l = NBlocks - NDirect ]].
+  Proof.
+    intros.
+    unfold indrep.
+    split; [> | cancel].
+    intros m' H'. pred_apply. cancel.
+    repeat rewrite <- plus_assoc. rewrite minus_plus.
+    indrep_n_tree_extract_lengths.
+    erewrite <- firstn_skipn with (l := l). rewrite app_length. f_equal; eauto.
+    erewrite <- firstn_skipn with (l := skipn _ _). rewrite app_length.
+    f_equal; eauto. rewrite skipn_skipn'. auto.
+  Qed.
+
+(*TODO move this *)
+  Theorem firstn_app_split : forall T (l1 l2 : list T) n,
+    firstn n (l1 ++ l2) = firstn n l1 ++ firstn (n - length l1) l2.
+  Proof.
+    intros.
+    destruct (le_lt_dec n (length l1)).
+    - rewrite firstn_app_l by auto.
+      replace (_ - _) with 0 by omega. rewrite app_nil_r. auto.
+    - rewrite firstn_app_le by omega.
+      f_equal. rewrite firstn_oob by omega. auto.
+  Qed.
+
+  Theorem indshrink_ok : forall lxp bxp ir nl ms,
+    {< F Fm m0 m l0 l1 l2 freelist,
+    PRE:hm
+           LOG.rep lxp F (LOG.ActiveTxn m0 m) ms hm * [[ nl <= length (l0 ++ l1 ++ l2) ]] *
+           [[[ m ::: (Fm * indrep_n_tree 0 bxp (IRIndPtr ir) l0 *
+                           indrep_n_tree 1 bxp (IRDindPtr ir) l1 *
+                           indrep_n_tree 2 bxp (IRTindPtr ir) l2 * BALLOC.rep bxp freelist) ]]]
+    POST:hm' RET:^(ms, indptr', dindptr', tindptr')
+           exists m' freelist' l0' l1' l2',
+           LOG.rep lxp F (LOG.ActiveTxn m0 m') ms hm' *
+           [[[ m' ::: (Fm * indrep_n_tree 0 bxp indptr' l0' *
+                            indrep_n_tree 1 bxp dindptr' l1' *
+                            indrep_n_tree 2 bxp tindptr' l2' * BALLOC.rep bxp freelist') ]]] *
+           [[ l0' ++ l1' ++ l2' = upd_range (l0 ++ l1 ++ l2) nl (length (l0 ++ l1 ++ l2) - nl) $0 ]] *
+           [[ incl freelist freelist' ]]
+    CRASH:hm'  LOG.intact lxp F m0 hm'
+    >} indshrink lxp bxp ir nl ms.
+  Proof.
+    unfold indshrink.
+    hoare.
+    repeat rewrite app_length in *.
+    indrep_n_tree_extract_lengths.
+    autorewrite with core.
+    unfold upd_range.
+    destruct (le_lt_dec nl NIndirect); [> |
+    destruct (le_lt_dec nl (NIndirect + NIndirect * NIndirect))];
+      repeat rewrite skipn_oob by (repeat rewrite app_length; omega);
+      repeat rewrite app_nil_r; repeat rewrite firstn_app_split;
+      repeat match goal with [|- context [?a - ?b] ] => 
+        replace (a - b) with 0 by omega end;
+      autorewrite with core; repeat rewrite <- app_assoc;
+      repeat rewrite repeat_app; repeat (omega || f_equal).
+  Qed.
+
+  Local Hint Extern 1 ({{_}} Bind (indshrink _ _ _ _ _) _) => apply indshrink_ok : prog.
 
   Theorem shrink_ok : forall lxp bxp ir nr ms,
     {< F Fm m0 m l freelist,
     PRE:hm
            LOG.rep lxp F (LOG.ActiveTxn m0 m) ms hm *
            [[[ m ::: (Fm * rep bxp ir l * BALLOC.rep bxp freelist) ]]]
-    POST:hm' RET:^(ms, r)  exists m' freelist',
+    POST:hm' RET:^(ms, r)  exists m' freelist' l',
            LOG.rep lxp F (LOG.ActiveTxn m0 m') ms hm' *
-           [[[ m' ::: (Fm * rep bxp r (cuttail nr l) * BALLOC.rep bxp freelist') ]]] *
-           [[ r = upd_len ir ((IRLen ir) - nr) ]] *
+           [[[ m' ::: (Fm * rep bxp r l' * BALLOC.rep bxp freelist') ]]] *
+           exists ind dind tind dirl, [[ r = upd_irec ir ((IRLen ir) - nr) ind dind tind dirl ]] *
+           [[ l' = firstn (IRLen ir - nr) l ]] *
            [[ incl freelist freelist' ]]
     CRASH:hm'  LOG.intact lxp F m0 hm'
     >} shrink lxp bxp ir nr ms.
   Proof.
     unfold shrink.
     prestep; norml.
-    assert (length l = (IRLen ir)); denote rep as Hx.
-    unfold rep in Hx; destruct_lift Hx; omega.
-
-    (* needs to free indirect block *)
-    prestep; norml.
-    rewrite rep_piff_indirect in Hx by omega.
-    unfold rep_indirect in Hx; destruct_lift Hx.
-    denote IndRec.rep as Hx; rewrite indrec_ptsto_pimpl in Hx.
-    destruct_lift Hx; cancel.
-
-    step.
-    rewrite rep_piff_direct by (rewrite cuttail_length; omega).
-    unfold rep_direct; cancel; autorewrite with core; try omega.
-    apply le_ndirect_goodSize; omega.
-
-    substl l at 1; unfold cuttail.
-    rewrite app_length, firstn_length_l by omega.
-    rewrite firstn_app_l by omega.
-    f_equal; omega.
-
-    (* no free indirect block *)
+    denote rep as Hx. unfold rep in Hx. destruct_lifts.
     cancel.
-
-    (* case 1: all in direct blocks *)
-    repeat rewrite rep_piff_direct by (autorewrite with core; omega).
-    unfold rep_direct; cancel; autorewrite with core; try omega.
-    apply le_ndirect_goodSize; omega.
-
-    substl l at 1; unfold cuttail.
-    rewrite firstn_length_l by omega.
-    rewrite firstn_firstn, Nat.min_l by omega; auto.
-
-    (* case 1: all in indirect blocks *)
-    repeat rewrite rep_piff_indirect by (autorewrite with core; omega).
-    unfold rep_indirect; cancel; autorewrite with core; eauto; try omega.
-    apply le_nblocks_goodSize; omega.
-
-    substl l at 1; unfold cuttail.
-    rewrite app_length, firstn_length_l by omega.
-    replace (length (IRBlocks ir) + (length l - NDirect) - nr) with
-            (length (IRBlocks ir) + (length l - nr - NDirect)) by omega.
-    rewrite firstn_app_r; f_equal.
-    rewrite firstn_firstn, Nat.min_l by omega; auto.
+    + (* case 1: all in direct blocks *)
+      step. unfold rep.
+      autorewrite with core. cancel.
+      apply upd_len_indrep.
+      rewrite min_l by omega. omega.
+      rewrite min_l by omega.
+      substl l at 1. rewrite firstn_firstn, min_l by omega. auto.
+      apply le_ndirect_goodSize. omega.
+      apply upd_irec_eq_upd_len. apply le_nblocks_goodSize. omega.
+    + (* case 2 : indirect blocks *)
+      unfold indrep in *.
+      hoare.
+      - repeat rewrite app_length.
+        indrep_n_tree_extract_lengths. omega.
+      - unfold rep, indrep. autorewrite with core; auto.
+        cancel; rewrite mult_1_r in *.
+        rewrite indrep_n_length_pimpl with (indlvl := 0).
+        rewrite indrep_n_length_pimpl with (indlvl := 1).
+        rewrite indrep_n_length_pimpl with (indlvl := 2). cancel. rewrite mult_1_r in *.
+        substl (NIndirect * NIndirect). substl NIndirect.
+        rewrite firstn_app. rewrite skipn_app_r. repeat rewrite skipn_app. rewrite firstn_app.
+        cancel.
+      all : try match goal with
+          | [|- goodSize _ ?a] =>
+            destruct (addr_eq_dec a 0); subst; [> apply DiskLogHash.PaddedLog.goodSize_0 |];
+            rewrite indrep_n_tree_valid with (ir := a) in * by auto;
+            rewrite BALLOC.bn_valid_goodSize_pimpl in *; destruct_lifts; intuition
+          | [|- _ ] => try rewrite min_l by omega; try omega
+          end.
+      all : indrep_n_tree_extract_lengths.
+      match goal with [H : _ ++ _ = _ |- _] => rewrite H end.
+      substl l. rewrite firstn_firstn, min_l by omega.
+      repeat rewrite firstn_app_split. f_equal.
+      rewrite firstn_upd_range by (repeat rewrite app_length; omega). f_equal.
+      rewrite <- skipn_skipn'.
+      repeat match goal with [|- ?x = _] =>
+        erewrite <- firstn_skipn with (l := x) at 1; f_equal end.
+      apply le_nblocks_goodSize. simpl. rewrite mult_1_r. omega.
   Qed.
 
+  (* TODO move this *)
+  Theorem repeat_eq_updN : forall T i (l : list T)  n v1 v2,
+    i < n ->
+    updN l i v1 = repeat v2 n -> v1 = v2.
+  Proof.
+    induction i; intros.
+    - destruct n. omega.
+      destruct l. simpl in *. inversion H0.
+      simpl in *. inversion H0; auto.
+    - destruct n. omega.
+      destruct l. simpl in *. inversion H0.
+      simpl in *. inversion H0.
+      eapply IHi; [> | eauto]. omega.
+  Qed.
+
+ Theorem indgrow_ok : forall lxp bxp ir off bn ms,
+    {< F Fm m0 m l0 l1 l2 freelist,
+    PRE:hm
+           LOG.rep lxp F (LOG.ActiveTxn m0 m) ms hm *
+           [[ off < NBlocks - NDirect ]] * [[ bn <> $0 ]] *
+           [[[ m ::: (Fm * indrep_n_tree 0 bxp (IRIndPtr ir) l0 *
+                           indrep_n_tree 1 bxp (IRDindPtr ir) l1 *
+                           indrep_n_tree 2 bxp (IRTindPtr ir) l2 * BALLOC.rep bxp freelist) ]]]
+    POST:hm' RET:^(ms, v, indptr', dindptr', tindptr')
+           exists m', LOG.rep lxp F (LOG.ActiveTxn m0 m') ms hm' *
+           ([[ v = 0 ]] \/ [[ v <> 0 ]] *
+           exists freelist' l0' l1' l2',
+           [[ updN (l0 ++ l1 ++ l2) (IRLen ir - NDirect) bn = l0' ++ l1' ++ l2' ]] *
+           [[[ m' ::: (Fm * indrep_n_tree 0 bxp indptr' l0' *
+                            indrep_n_tree 1 bxp dindptr' l1' *
+                            indrep_n_tree 2 bxp tindptr' l2' * BALLOC.rep bxp freelist') ]]] *
+           [[ incl freelist' freelist ]])
+    CRASH:hm'  LOG.intact lxp F m0 hm'
+    >} indgrow lxp bxp ir off bn ms.
+  Proof.
+    unfold indgrow. prestep. norml.
+    indrep_n_tree_extract_lengths.
+    hoare.
+    all : or_r; cancel.
+    all : match goal with
+          | [|- _ = _ ] =>
+            repeat rewrite updN_app2 by omega; try rewrite updN_app1 by omega; congruence
+          | [H : ?a = 0, H' : context [indrep_n_tree _ _ ?a _] |- _] =>
+            rewrite H in H'; rewrite indrep_n_tree_0 in H'; destruct_lifts; rewrite mult_1_r in *;
+            match goal with [H : updN _ _ _ = repeat _ _ |- _] => 
+              apply repeat_eq_updN in H; [> contradiction | omega] end
+          end.
+  Qed.
+
+  Local Hint Extern 1 ({{_}} Bind (indgrow _ _ _ _ _) _) => apply indgrow_ok : prog.
+
+(* TODO move this *)
+Local Hint Extern 1 (goodSize _ _) => match goal with
+| [|- goodSize _ ?a] =>
+  destruct (addr_eq_dec a 0); [> substl a; apply DiskLogHash.PaddedLog.goodSize_0 |];
+  rewrite indrep_n_tree_valid with (ir := a) in * by auto; destruct_lifts;
+  eapply BALLOC.bn_valid_goodSize; eassumption
+end.
 
   Theorem grow_ok : forall lxp bxp ir bn ms,
     {< F Fm m0 m l freelist,
@@ -2729,12 +2962,12 @@ Hint Rewrite le_plus_minus_r using auto.
            [[ length l < NBlocks ]] *
            [[[ m ::: (Fm * rep bxp ir l * BALLOC.rep bxp freelist) ]]]
     POST:hm' RET:^(ms, r)
-           [[ r = None ]] * LOG.rep lxp F (LOG.ActiveTxn m0 m) ms hm' \/
-           exists m' freelist' ir',
+           exists m',
+           [[ r = None ]] * LOG.rep lxp F (LOG.ActiveTxn m0 m') ms hm' \/
+           exists freelist' ir',
            [[ r = Some ir' ]] * LOG.rep lxp F (LOG.ActiveTxn m0 m') ms hm' *
            [[[ m' ::: (Fm * rep bxp ir' (l ++ [bn]) * BALLOC.rep bxp freelist') ]]] *
-           [[ IRAttrs ir' = IRAttrs ir /\ length (IRBlocks ir') = length (IRBlocks ir) ]] *
-           [[ incl freelist' freelist ]]
+           [[ IRAttrs ir' = IRAttrs ir /\ length (IRBlocks ir') = length (IRBlocks ir) ]]
     CRASH:hm'  LOG.intact lxp F m0 hm'
     >} grow lxp bxp ir bn ms.
   Proof.
@@ -2752,66 +2985,75 @@ Hint Rewrite le_plus_minus_r using auto.
     rewrite rep_piff_direct by (autorewrite with lists; simpl; omega).
     unfold rep_direct; autorewrite with core lists; simpl.
     cancel; try omega.
-    substl l at 1; substl (length l).
+    unfold indrep.
+    intros m' H'. pred_apply. autorewrite with core. cancel.
+    all : try match goal with
+    | [|- goodSize _ ?a] =>
+      destruct (addr_eq_dec a 0); [> substl a; apply DiskLogHash.PaddedLog.goodSize_0 |];
+      rewrite indrep_n_tree_valid with (ir := a) in * by auto; destruct_lifts;
+      eapply BALLOC.bn_valid_goodSize; eassumption
+    end.
+    substl l at 1. substl (length l).
     apply firstn_app_updN_eq; omega.
     apply le_nblocks_goodSize; omega.
     autorewrite with core lists; auto.
 
     (* update indirect blocks *)
     step.
-    step.
-
-    (* case 1 : need allocate indirect block *)
-    step; try (eapply BALLOC.bn_valid_facts; eauto).
-    unfold IndSig.xparams_ok; auto.
-    instantiate (1 := [(dummy_cur, dummy_old)]); simpl; auto.
-    simpl; unfold IndSig.RAStart; cancel.
-
-    step.
-    rewrite repeat_length; omega.
-    step.
-    or_r; cancel.
-    rewrite rep_piff_direct by omega.
-    rewrite rep_piff_indirect by (rewrite app_length; simpl; omega).
-    unfold rep_direct, rep_indirect; cancel;
-      repeat (autorewrite with core lists; simpl; eauto; try omega).
-    eapply BALLOC.bn_valid_goodSize; eauto.
-    apply le_nblocks_goodSize; omega.
-    eapply BALLOC.bn_valid_goodSize; eauto.
-
-    substl l at 1; substl (length l); substl (IRLen ir).
-    rewrite firstn_oob, minus_plus, Nat.sub_diag by omega.
-    erewrite firstn_S_selN, selN_updN_eq by (autorewrite with lists; omega).
-    simpl; auto.
-    autorewrite with core lists; auto.
-
-    apply incl_remove.
-
-    (* case 2 : just update the indirect block *)
-    prestep; norml.
-    rewrite rep_piff_indirect in Hx by omega.
-    unfold rep_indirect in Hx; destruct_lift Hx; cancel; try omega.
-    2: cancel.
-    omega.
-
-    step.
-    or_r; cancel.
-    rewrite rep_piff_indirect by (rewrite app_length; simpl; omega).
-    unfold rep_indirect; cancel;
-      repeat (autorewrite with core lists; simpl; eauto; try omega).
-    eapply BALLOC.bn_valid_goodSize; eauto.
-    apply le_nblocks_goodSize; omega.
-    eapply BALLOC.bn_valid_goodSize; eauto.
-    substl l at 1; substl (length l).
-    replace (IRLen ir + 1 - NDirect) with (IRLen ir - NDirect + 1) by omega.
-    rewrite <- app_assoc; f_equal.
-    rewrite firstn_app_updN_eq; auto.
-    substl (length dummy); omega.
-    autorewrite with core lists; auto.
-
-    cancel.
-
-    Unshelve. all:eauto.
+    + (* write 0 block *)
+      unfold rep in *. destruct_lifts.
+      rewrite indrep_length_pimpl in *. unfold indrep in *. destruct_lifts.
+      indrep_n_tree_extract_lengths.
+      hoare.
+      - repeat rewrite app_length. omega.
+      - rewrite <- skipn_skipn' in *. repeat rewrite firstn_skipn in *.
+        indrep_n_tree_extract_lengths.
+        or_r; cancel; autorewrite with core; (cancel || auto).
+        rewrite <- skipn_skipn'.
+        rewrite firstn_app. rewrite skipn_app_l. rewrite skipn_oob. rewrite app_nil_l.
+        rewrite firstn_app. rewrite skipn_app_l. rewrite skipn_oob. rewrite app_nil_l.
+        cancel_last.
+        all : try rewrite app_length; simpl; try omega.
+       -- apply le_nblocks_goodSize. simpl. rewrite mult_1_r. omega.
+       -- substl l at 1.
+          rewrite plus_comm.
+          repeat match goal with [|- context [firstn ?a (?b ++ ?c)] ] =>
+            rewrite firstn_app_split with (l1 := b); rewrite firstn_oob with (l := b) by omega
+          end. rewrite <- app_assoc. f_equal.
+          rewrite Nat.sub_succ_l by omega.
+          match goal with [H : _ ++ _ = _ |- _] => rewrite H end.
+          erewrite firstn_S_selN.
+          rewrite firstn_upd_range by omega. f_equal.
+          rewrite upd_range_selN by omega. auto.
+          rewrite upd_range_length; omega.
+    + (* write nonzero block *)
+      unfold rep in *. destruct_lifts.
+      rewrite indrep_length_pimpl in *. unfold indrep in *. destruct_lifts.
+      indrep_n_tree_extract_lengths.
+    (* TODO update this above *)
+      Local Hint Extern 1 ({{_}} Bind (indgrow _ _ _ _ _ _) _) => apply indgrow_ok : prog.
+      hoare.
+      - rewrite mult_1_r. omega.
+      - rewrite <- skipn_skipn' in *. repeat rewrite firstn_skipn in *.
+        indrep_n_tree_extract_lengths.
+        or_r. cancel; autorewrite with core.
+        rewrite <- skipn_skipn'.
+        rewrite firstn_app. rewrite skipn_app_l. rewrite skipn_oob. rewrite app_nil_l.
+        rewrite firstn_app. rewrite skipn_app_l. rewrite skipn_oob. rewrite app_nil_l.
+        (* TODO make this unnecessary by fixing cancel_last to not use pimpl_refl *)
+        rewrite sep_star_assoc. rewrite sep_star_comm with (p1 := indrep_n_tree 1 _ _ _). cancel_last.
+        all : repeat rewrite app_length; try solve [auto | simpl; omega].
+       -- apply le_nblocks_goodSize. simpl. rewrite mult_1_r. omega.
+       -- rewrite plus_comm.
+          match goal with [H : updN _ _ _ = _ |- _] => rewrite <- H end.
+          erewrite firstn_S_selN. substl l at 1.
+          repeat rewrite firstn_app_le by omega.
+          rewrite firstn_updN_oob by omega. rewrite selN_app2 by omega.
+          erewrite eq_trans with (x := _ - _); [> | reflexivity |].
+          rewrite selN_updN_eq by omega. reflexivity.
+          all : try rewrite app_length, length_updN; omega.
+    Grab Existential Variables.
+    all : eauto; exact $0.
   Qed.
 
   Hint Extern 1 ({{_}} Bind (get _ _ _ _) _) => apply get_ok : prog.
